## 4. Sean las cadenas $\alpha=abb$ y $\beta=acb$. Calcular:

### a) $\alpha\beta$

Por definición
$$
    \alpha\beta = abbacb
$$

### b) $(\alpha\beta)^r$

Por definición
$$
    (\alpha\beta)^r = (abbacb)^r = bcabba
$$

### c) $\beta^r$

Por definición
$$
    \beta^r = bca
$$

### d) $\beta^r\alpha^r$

Por definición
$$
    \beta^r\alpha^r = bcabba
$$

### e) $\lambda\alpha$

Por definición
$$
    \lambda\alpha = \alpha = abb
$$

### f) $\lambda\beta$

Por definición
$$
    \lambda\beta = \beta = acb
$$

### g) $\alpha\lambda\beta$

Por definición
$$
    \alpha\lambda\beta = \alpha\beta = abbacb
$$

### h) $\alpha^2\lambda^3\beta^2$

Por definición
$$
    \alpha^2\lambda^3\beta^2 = abbabbacbacb
$$
